computation

LeanScratch/Computation/RegMachine.lean
@@ -1,37 +1,72 @@
 import LeanScratch.Vec
 import LeanScratch.Fin2
 
-def Vec.zeros : (n : Nat) → Vec Nat n
-  | 0 => %[]
-  | _+1 => 0 %:: Vec.zeros _
-
 namespace Comp
 
+inductive RegTree
+  | lf (n : Nat)
+  | br (l r : RegTree)
+
+abbrev RegTree.toStore : RegTree → Type
+  | .lf n => Vec Nat n
+  | .br l r => l.toStore × r.toStore
+
+def Vec.zero {n} : Vec Nat n :=
+  match n with
+  | 0 => %[]
+  | _+1 => 0 %::zero
+
+def RegTree.toStore.zero {r : RegTree} : r.toStore :=
+  match r with
+  | .lf _ => Vec.zero
+  | .br _ _ => ⟨zero, zero⟩
+
+instance {r : RegTree} : Repr r.toStore where
+  reprPrec v _ := f v
+    where
+      f {r : RegTree} (v : r.toStore) : Std.Format := match r with
+      | .lf _ => repr v
+      | .br _ _ => .bracket "⟨" (f v.fst ++ ", " ++ f v.snd) "⟩"
+
+abbrev RegTree.toIdx : RegTree → Type
+  | .lf n => Fin2 n
+  | .br l r => l.toIdx ⊕ r.toIdx
+
 -- Observation: any sequence of inc steps can be compressed into one large multi-reg inc
-inductive RegMachine.Ins (r : Nat) (L : Type)
-  | inc (r : Fin2 r) (l : L)
-  | dec (r : Fin2 r) (l1 l2 : L)
+inductive RegMachine.Ins (r : RegTree) (L : Type)
+  | inc (r : r.toIdx) (l : L)
+  | dec (r : r.toIdx) (nzdest zdest : L)
   | hlt
 
-def RegMachine (r : Nat) (L : Type) := L → RegMachine.Ins r L
+def RegMachine (r : RegTree) (L : Type) := L → RegMachine.Ins r L
 
 namespace RegMachine
 
-structure Config (r : Nat) (L : Type) :=
-  regs : Vec Nat r
+structure Config (r : RegTree) (L : Type) :=
+  regs : r.toStore
   state : L
 deriving Repr
 
 variable (machine : RegMachine r L)
 
-def inc {r} : Fin2 r → Vec Nat r → Vec Nat r
+def inc_vec {r} : Fin2 r → Vec Nat r → Vec Nat r
   | .fz, hd %:: tl => (hd + 1) %:: tl
-  | .fs n, hd %:: tl => hd %:: inc n tl
+  | .fs n, hd %:: tl => hd %:: inc_vec n tl
 
-def dec {r} : Fin2 r → Vec Nat r → Option (Vec Nat r)
+def inc : {r : RegTree} → r.toIdx → r.toStore → r.toStore
+  | .lf _, idx, str => inc_vec idx str
+  | .br _ _, .inl search, ⟨a, b⟩ => ⟨inc search a, b⟩
+  | .br _ _, .inr search, ⟨a, b⟩ => ⟨a, inc search b⟩
+
+def dec_vec {r} : Fin2 r → Vec Nat r → Option (Vec Nat r)
   | .fz, 0 %:: tl => .none
   | .fz, hd + 1 %:: tl => .some (hd %:: tl)
-  | .fs n, hd %:: tl => dec n tl |>.map (.cons hd)
+  | .fs n, hd %:: tl => dec_vec n tl |>.map (.cons hd)
+
+def dec : {r : RegTree} → r.toIdx → r.toStore → Option r.toStore
+  | .lf _, idx, str => dec_vec idx str
+  | .br _ _, .inl search, ⟨a, b⟩ => (dec search a).map (⟨·, b⟩)
+  | .br _ _, .inr search, ⟨a, b⟩ => (dec search b).map (⟨a, ·⟩)
 
 def Config.step (state : Config r L) : Option $ Config r L :=
   let ⟨regs, state⟩ := state
@@ -47,37 +82,92 @@ def Config.step_n (state : Config r L) : Nat → Option (Config r L)
   | 0 => state
   | n+1 => (state.step machine).bind (step_n · n)
 
+
+def Config.step_n.add {start : Config r L} : start.step_n machine (a + b) = (start.step_n machine b).bind (·.step_n machine a) :=
+  match b with
+  | 0 => rfl
+  | n+1 => by
+    dsimp [step_n]
+    by_cases h : ∃ w, (step machine start) = .some w
+    · rcases h with ⟨w, p⟩
+      simp only [p, Option.some_bind]
+      exact step_n.add
+    · simp only [← Option.ne_none_iff_exists', ne_eq, not_not] at h
+      simp only [Option.none_bind, h]
+
 def Config.trace (state : Config r L): Nat → List (Config r L)
   | 0 => []
   | n+1 => state :: match state.step machine with
     | .some next => next.trace n
     | .none => []
 
-def TerminatesWith (start term : Config r L) : Prop :=
+def StepsTo (start conn : Config r L) : Prop :=
+  ∃ n, start.step_n machine n = .some conn
+
+namespace StepsTo
+
+theorem step
+    (x : a.step machine = .some b)
+    (h : StepsTo machine b c)
+    : StepsTo machine a c := by
+  rcases h with ⟨w, hb⟩
+  refine ⟨w.succ, ?_⟩
+  simp only [Config.step_n, x, Option.some_bind, hb]
+
+def trans {m} : StepsTo m a b → StepsTo m b c → StepsTo m a c
+  | ⟨w₁, p₁⟩, ⟨w₂, p₂⟩ =>
+    ⟨w₂ + w₁, by simp only [Config.step_n.add, p₁, Option.some_bind, p₂] ⟩
+
+instance {m : RegMachine r L} : Trans (StepsTo m) (StepsTo m) (StepsTo m) := ⟨trans⟩
+
+def refl : StepsTo machien a a := ⟨0, rfl⟩
+
+end StepsTo
+
+/-- Terminates with -/
+def TW (start term : Config r L) : Prop :=
   ∃ n, start.step_n machine n = .some term ∧ term.step machine = .none
 
-theorem TerminatesWith_step
-    machine (x : a.step machine = .some b)
-    (h : TerminatesWith machine b c)
-    : TerminatesWith machine a c := by
+namespace TW
+
+def trans {m} : StepsTo m a b → TW m b c → TW m a c
+  | ⟨w₁, p₁⟩, ⟨w₂, p₂, p₃⟩ =>
+    ⟨w₂ + w₁, by simp [Config.step_n.add, p₁, p₂, p₃]⟩
+
+instance {m : RegMachine r L} : Trans (StepsTo m) (TW m) (TW m) := ⟨trans⟩
+
+theorem step
+    (x : a.step machine = .some b)
+    (h : TW machine b c)
+    : TW machine a c := by
   rcases h with ⟨w, ha, hb⟩
   refine ⟨w.succ, ?_, hb⟩
   simp only [Config.step_n, x, Option.some_bind]
   exact ha
 
-theorem TerminatesWith_rfl machine (h : a.step machine = .none) : TerminatesWith machine a a := ⟨0, rfl, h⟩
+theorem refl (h : a.step machine = .none) : TW machine a a := ⟨0, rfl, h⟩
+
+end TW
+
+/- theorem TW_drive_lemma machine (correct : TW machine b c) : a.state = b.state → a.regs = b.regs → TW machine a c := -/
+/-   fun seq regeq => match a, b with -/
+/-     | ⟨ar, as⟩, ⟨br, bs⟩ => by simp_all only -/
 
 end RegMachine
 
-/- def Computable (f : Vec Nat ina → Vec Nat outa) : Prop := -/
-/-   ∃ regc L s, ∃ m : RegMachine (outa + ina + regc) L, -/
-/-     ∀ inp, ∃ (rst : Vec _ _), ∃ e, m.TerminatesWith ⟨padderA inp, s⟩ ⟨padderB (f inp), e⟩ -/
-/-   where -/
-/-     padderA {regc l} (ls : Vec Nat l) : Vec Nat (outa + l + regc) := -/
-/-       match ls, regc with -/
-/-       | _, 0   => sorry -/
-/-       | z, n+1 => 0 %:: padderA z -/
-/-     padderB {regc other l} (ls : Vec Nat l) :  Vec Nat (l + other + regc) := -/
-/-       match ls, regc with -/
-/-       | _, _ => sorry -/
+macro "drive" "TW" : tactic => `(tactic|
+    repeat apply $(Lean.mkIdent ``RegMachine.TW.step) _ (by rfl); try {exact $(Lean.mkIdent ``RegMachine.TW.refl)      _ (by rfl)}
+  )
+macro "drive" "StepsTo" : tactic => `(tactic|
+    repeat apply $(Lean.mkIdent ``RegMachine.StepsTo.step) _ (by rfl); try {apply $(Lean.mkIdent ``RegMachine.StepsTo.refl) }
+  )
+-- TODO
+/- macro "drive" "with" term:term : tactic => `(tactic | { -/
+/-   repeat apply RegMachine.TW_step _ (by rfl) -/
+/-   apply RegMachine.TW_drive_lemma _ $term rfl -/
+/- }) -/
 
+class Computable (f : Vec Nat ina → Vec Nat outa) : Prop :=
+  computable : ∃ L r, ∃ m : RegMachine (.br (.lf outa) $ .br (.lf ina) r) L,
+    ∃ starts, ∀ inp : Vec Nat ina, ∃ e ends, m.TW
+      ⟨⟨.zero, ⟨inp, .zero⟩⟩, starts⟩ ⟨⟨f inp, e⟩, ends⟩
